directed to undircted

reduction_directedHamiltonianCircuit_to_hamiltonianCircuit3.dfy
@@ -1,6 +1,6 @@
 type Graph = seq<seq<bool>>
 
-//squared and triangular matrix
+//squared and triangular superior matrix
 ghost predicate validUndirectedGraph(g: Graph)
 {
     (forall s :: s in g ==> |s|==|g|) &&
@@ -71,14 +71,64 @@ ghost predicate hamiltonianCircuitPartialCorrectness(g: Graph, circuit: seq<nat>
 The reduction:
  */
 
+/////// AUXILIAR PREDICATES //////
+
+ghost predicate unconnected_graph(g: Graph)
+    requires validGraph(g)
+{
+    forall f :: 0<=f<|g| ==> (forall c :: 0<=c<|g| ==> !g[f][c])
+}
+
+//original nodes are only adjacent to their respective out and in nodes and there are only out->in vertex
+ghost predicate in_out_graph(g: Graph, s: int)
+    requires validUndirectedGraph(g)
+    requires |g|==s*3
+{
+    forall f :: 0<=f< s ==> (forall c :: 0<=c<|g| ==>
+        (
+            ((c==f+s || c==f+s*2) ==> g[f][c])     //out node: i+s, in node: i+s*2
+            &&
+            ((c!=f+s && c!=f+s*2) ==> !g[f][c])    //rest: false (original nodes are not interconnected)
+        )
+    )
+    &&
+    (forall f :: s<=f< s*2 ==> (forall c :: s<=c< s*2 ==> !g[f][c]))    //no vertex from out to out
+    &&
+    (forall f :: s*2<=f< s*3 ==> (forall c :: s*2<=c< s*3 ==> !g[f][c]))    //no vertex from in to in
+}
+
+ghost predicate unconnected_in_out_graph(g: Graph, s: int)
+    requires validUndirectedGraph(g)
+    requires |g|==s*3
+{
+    in_out_graph(g, s)
+    &&
+    forall f :: s<=f<|g| ==> (forall c :: 0<=c<|g| ==> !g[f][c])
+}
+
+ghost predicate out_node_unconnected(g: Graph, g0: Graph, n: int)
+    requires validUndirectedGraph(g)
+    requires |g|==|g0|*3
+    requires 0<=n< |g0|
+{
+    forall c :: 0<=c< |g| ==> !g[n+|g0|][c] //no vertex for n_out node
+}
+
+/////// REDUCTION FUNCTION ///////
+
 ghost function directed_to_undirected_graph(g: Graph): Graph
     requires |g|>0
     requires validGraph(g)
-    // ensures directed(validUndirectedGraph(g))
+    //size relation
+    ensures |directed_to_undirected_graph(g)| == |g|*3
+    //squared and triangular superior matrix
+    ensures validUndirectedGraph(directed_to_undirected_graph(g))
+    //original nodes are only adjacent to their respective out and in nodes and there are only out->in vertex
+    ensures in_out_graph(directed_to_undirected_graph(g), |g|)
+    //direction relation: n1->n2 in g only and only if n1_out-n2_in in g'
+    ensures forall f :: 0<=f<|g| ==> (forall c :: 0<=c<|g| ==> (g[f][c] <==> directed_to_undirected_graph(g)[f+|g|][c+|g|*2]))
 {
-    var eg := extended_graph(g);
-    var io := in_out_nodes(eg, |g|);
-    direction_equivalence(g, io)
+    direction_equivalence(g, in_out_nodes(extended_graph(g), |g|))
 }
 
 ghost function extended_graph(g: Graph): Graph
@@ -99,7 +149,6 @@ ghost function in_out_nodes(g: Graph, s: int): Graph
     ensures |in_out_nodes(g, s)| == |g|
     ensures validUndirectedGraph(in_out_nodes(g, s))
     ensures unconnected_in_out_graph(in_out_nodes(g, s), s)
-    ensures forall f :: s<=f<|g| ==> (forall c :: 0<=c<|g| ==> !in_out_nodes(g, s)[f][c])
 {
     in_out_nodes_(g, s, s-1)
 }
@@ -113,8 +162,6 @@ ghost function in_out_nodes_(g: Graph, s: int, i: int): Graph
     decreases i
     ensures |in_out_nodes_(g, s, i)| == |g|
     ensures validUndirectedGraph(in_out_nodes_(g, s , i))
-    // ensures forall f :: 0<=f<=i ==> in_out_nodes_(g, s, i)[f][f+s] && in_out_nodes_(g, s, i)[f][f+s*2]
-    // ensures forall f :: 0<=f<=i ==> !(exists c :: 0<=c<|g| && c!=f+s && c!=f+s*2 && !in_out_nodes_(g, s, i)[f][c])
     ensures forall f :: i< f<|g| ==> (forall c :: 0<=c<|g| ==> !in_out_nodes_(g, s, i)[f][c])
     ensures forall f :: 0<=f<=i ==> (forall c :: 0<=c<|g| ==>
         (
@@ -132,44 +179,20 @@ ghost function in_out_nodes_(g: Graph, s: int, i: int): Graph
         g'[i:=f'']
 }
 
-//auxiliar predicates:
-ghost predicate unconnected_graph(g: Graph)
-    requires validGraph(g)
-{
-    forall f :: 0<=f<|g| ==> (forall c :: 0<=c<|g| ==> !g[f][c])
-}
-
-ghost predicate unconnected_in_out_graph(g: Graph, s: int)
-    requires validUndirectedGraph(g)
-    requires |g|==s*3
-{
-    forall f :: 0<=f< s ==> (forall c :: 0<=c<|g| ==>
-        (
-            ((c==f+s || c==f+s*2) ==> g[f][c])     //out node: i+s, in node: i+s*2
-            &&
-            ((c!=f+s && c!=f+s*2) ==> !g[f][c])    //rest: false
-        )
-    )
-    &&
-    forall f :: s<=f<|g| ==> (forall c :: 0<=c<|g| ==> !g[f][c])
-}
-
-ghost predicate out_node_unconnected(g: Graph, g0: Graph, n: int)
-    requires validUndirectedGraph(g)
-    requires |g|==|g0|*3
-    requires 0<=n< |g0|
-{
-    forall c :: 0<=c< |g| ==> !g[n+|g0|][c] //no tiene nodos salientes
-    // &&
-    // (forall c :: 0<=c<|g| ==> !g[n+s*2][c])
-}
-
 ghost function direction_equivalence(g: Graph, g': Graph): Graph
     requires |g|>0
     requires validGraph(g)
     requires validUndirectedGraph(g')
     requires |g'|==|g|*3
     requires unconnected_in_out_graph(g', |g|)
+    //size persistence
+    ensures |direction_equivalence(g, g')| == |g'|
+    //squared and triangular superior matrix
+    ensures validUndirectedGraph(direction_equivalence(g, g'))
+    //original nodes are only adjacent to their respective out and in nodes and there are only out->in vertex
+    ensures in_out_graph(direction_equivalence(g, g'), |g|)
+    //modifying property: n1->n2 in g only and only if n1_out-n2_in in g'
+    ensures forall f :: 0<=f<|g| ==> (forall c :: 0<=c<|g| ==> (g[f][c] <==> direction_equivalence(g, g')[f+|g|][c+|g|*2]))
 {
     direction_equivalence_(g, g', |g|-1)
 }
@@ -180,11 +203,25 @@ ghost function direction_equivalence_(g: Graph, g': Graph, i: int): Graph
     requires validUndirectedGraph(g')
     requires |g'|==|g|*3
     requires -1<=i<|g|
+    requires unconnected_in_out_graph(g', |g|)
+    ensures |direction_equivalence_(g, g', i)| == |g'|
+    ensures validUndirectedGraph(direction_equivalence_(g, g', i))
+    //only out nodes are modified (original nodes and in nodes stay the same)
+    ensures forall f :: 0<=f<|g| ==> (g'[f] == direction_equivalence_(g, g', i)[f])
+    ensures forall f :: |g|*2<=f<|g'| ==> (g'[f] == direction_equivalence_(g, g', i)[f])
+    //only out to in vertex are modified so vertex in the range [0]..[|g|*2-1] stay the same
+    ensures forall f :: |g|<=f<|g|*2 ==> (forall c :: 0<=c<|g|*2 ==> (g'[f][c] == direction_equivalence_(g, g', i)[f][c]))
+    //inductive postconditions
+    //every row yet to process stay the same
+    ensures forall f :: i+|g|< f<|g'| ==> (g'[f] == direction_equivalence_(g, g', i)[f])
+    //modifying property: for every processed row: n_out to c_in in g' if and only if n to c in g
+    ensures forall f :: 0<=f<=i ==> (forall c :: 0<=c<|g| ==> (g[f][c] <==> direction_equivalence_(g, g', i)[f+|g|][c+|g|*2]))
 {
     if i==-1 then g' else
         var g'' := direction_equivalence_(g, g', i-1);
-        //recorrer fila: si columna es true entonces [columna+s](out)[fila+s*2](in) := true
-        g''
+        //recorrer fila: si columna es true entonces [fila+s](out)[columna+s*2](in) := true
+        var gF := direction_equivalence_node(g, g'', i);
+        gF
 }
 
 ghost function direction_equivalence_node(g: Graph, g': Graph, n: int): Graph
@@ -194,6 +231,15 @@ ghost function direction_equivalence_node(g: Graph, g': Graph, n: int): Graph
     requires |g'|==|g|*3
     requires 0<=n<|g|
     requires out_node_unconnected(g', g, n)
+    ensures |direction_equivalence_node(g, g', n)| == |g'|
+    ensures validUndirectedGraph(direction_equivalence_node(g, g', n))
+    //only n_out's row is modified
+    ensures forall f :: 0<=f<|g'| && f!=n+|g| ==> (g'[f] == direction_equivalence_node(g, g', n)[f])
+    //only n_out to x_in vertex are modified, so columns below n+|g|*2 stay the same (set to false)
+    ensures forall c :: 0<=c<|g|*2 ==> (g'[n+|g|][c] == direction_equivalence_node(g, g', n)[n+|g|][c])
+    ensures forall c :: 0<=c<|g|*2 ==> !direction_equivalence_node(g, g', n)[n+|g|][c]
+    //modifying property: n_out to c_in in g' if and only if n to c in g
+    ensures forall c :: 0<=c<|g| ==> (g[n][c] <==> direction_equivalence_node(g, g', n)[n+|g|][c+|g|*2])
 {
     direction_equivalence_node_(g, g', n, |g|-1)
 }
@@ -209,89 +255,37 @@ columna i del nodo n en g:
 ghost function direction_equivalence_node_(g: Graph, g': Graph, n: int, i: int): Graph
     requires |g|>0
     requires validGraph(g)
-    requires validGraph(g')
-    requires |g'|==|g|*3
     requires validUndirectedGraph(g')
+    requires |g'|==|g|*3
     requires 0<=n<|g|
     requires -1<=i<|g|
     requires out_node_unconnected(g', g, n)
     ensures |direction_equivalence_node_(g, g', n, i)| == |g'|
     ensures validUndirectedGraph(direction_equivalence_node_(g, g', n, i))
-    // ensures forall 
-    // ensures forall f :: i< f<|g| ==> (g'[n+|g|][f+|g|*2] == direction_equivalence_node_(g, g', n, i)[n+|g|][f+|g|*2])
-    // ensures forall f :: i< f<|g| ==> !direction_equivalence_node_(g, g', n, i)[n+|g|][f+|g|*2]
-    // ensures i>=0 ==> (g[n][i] <==> direction_equivalence_node_(g, g', n, i)[n+|g|][i+|g|*2]) //no prueba la vuelta
-    // ensures forall c :: 0<=c<=i ==>
-    // (
-    //     g[n][c] <==> direction_equivalence_node_(g, g', n, i)[n+|g|][c+|g|*2]
-    // )
-{
-    if i==-1 then
-        assert out_node_unconnected(g', g, n);
-        assert !g'[n+|g|][i+|g|*2];
-        assert forall f :: i< f<|g| ==> !g'[n+|g|][f+|g|*2];
-        g'
-    else
-        var g'' := direction_equivalence_node_(g, g', n, i-1);
-        // assert !g''[n+|g|][i+|g|*2];
-        // assert forall f :: i<= f<|g| ==> !g''[n+|g|][f+|g|*2];
-        //recorrer fila: si columna es true entonces [n+s](n_out)[i+s*2](i_in) := true
-        if g[n][i] then
-            var f_aux1 := g''[n+|g|];
-            var f_aux2 := f_aux1[..i+|g|*2]+[true]+f_aux1[i+|g|*2+1..];
-            // assert forall f :: i< f<|g| ==> !f_aux2[f+|g|*2];
-            g''[n+|g| := f_aux2]
-        else
-            // assert out_nodes_unconnected(g', g, n);
-            // assume forall c :: 0<=c<|g| ==> !g'[n+|g|][c+2*|g|];
-            // assert !g''[n+|g|][i+|g|*2];    //ESTO: si !arista(n,i) -> !arista(n_out,i_in)
-            // assert forall f :: i< f<|g| ==> g''[n+|g|][f+|g|*2];
-            g''
-}
-
-lemma direction_equivalence_node_lemma1(g: Graph, g': Graph, n: int, i: int)
-    requires |g|>0
-    requires validGraph(g)
-    requires validGraph(g')
-    requires |g'|==|g|*3
-    requires validUndirectedGraph(g')
-    requires 0<=n<|g|
-    requires -1<=i<|g|-1
-    requires out_node_unconnected(g', g, n)
+    //only n_out's row is modified
+    ensures forall f :: 0<=f<|g'| && f!=n+|g| ==> (g'[f] == direction_equivalence_node_(g, g', n, i)[f])
+    //only n_out -> x_in vertex are modified, so columns below n+|g|*2 stay the same
+    ensures forall c :: 0<=c<|g|*2 ==> (g'[n+|g|][c] == direction_equivalence_node_(g, g', n, i)[n+|g|][c])
+    //inductive postconditions:
+    //every column yet to process stays the same (set to false)
+    ensures forall f :: i+|g|*2< f<|g'| ==> (g'[n+|g|][f] == direction_equivalence_node_(g, g', n, i)[n+|g|][f])
+    ensures forall f :: i< f<|g| ==> (g'[n+|g|][f+|g|*2] == direction_equivalence_node_(g, g', n, i)[n+|g|][f+|g|*2])
+    ensures forall f :: i< f<|g| ==> !direction_equivalence_node_(g, g', n, i)[n+|g|][f+|g|*2]
+    //modifying property: n_out to i_in in g' if and only if n to c in g
     ensures forall c :: 0<=c<=i ==>
     (
         g[n][c] <==> direction_equivalence_node_(g, g', n, i)[n+|g|][c+|g|*2]
     )
 {
-    if i>0
-    {
-        direction_equivalence_node_lemma1(g, g', n, i-1);
-        direction_equivalence_node_lemma2(g, g', n, i);
-        if g[n][i]
-        {
-            assume forall c :: 0<=c<=i ==>
-            (
-                g[n][c] <==> direction_equivalence_node_(g, g', n, i)[n+|g|][c+|g|*2]
-            );
-        }
+    if i==-1 then
+        g'
+    else
+        var g'' := direction_equivalence_node_(g, g', n, i-1);
+        if g[n][i] then
+            var f_aux1 := g''[n+|g|];
+            var f_aux2 := f_aux1[..i+|g|*2]+[true]+f_aux1[i+|g|*2+1..];
+            var gF := g''[n+|g| := f_aux2];
+            gF
         else
-        {
-            var g'' := direction_equivalence_node_(g, g', n, i-1);
-            direction_equivalence_node_lemma2(g, g', n, i-1);
-            assert direction_equivalence_node_(g, g', n, i) == g'';
-            assert forall f :: i<= f<|g| ==> !g''[n+|g|][f+|g|*2];
-        }
-    }
+            g''
 }
-
-lemma direction_equivalence_node_lemma2(g: Graph, g': Graph, n: int, i: int)
-    requires |g|>0
-    requires validGraph(g)
-    requires validGraph(g')
-    requires |g'|==|g|*3
-    requires validUndirectedGraph(g')
-    requires 0<=n<|g|
-    requires -1<=i<|g|-1
-    requires out_node_unconnected(g', g, n)
-    ensures forall f :: i< f<|g| ==> !direction_equivalence_node_(g, g', n, i)[n+|g|][f+|g|*2]
-{}
